proof/extraction/XMSS_IMPL_HOP1.ec
@@ -18,7 +18,7 @@ op Hash_ptr : W64.t -> W64.t -> W8.t Array32.t.
 
 op _PRF_ : W8.t Array32.t -> W8.t Array32.t -> W8.t Array32.t -> W8.t Array32.t.
 
-op _PRF_KEYGEN_ : W8.t list -> W8.t list -> W8.t list.
+op _PRF_KEYGEN_ : W8.t Array64.t -> W8.t Array32.t -> W8.t Array32.t.
 
 module M_Hop1(SC:Syscall_t) = {
   proc __u32_to_bytes (out:W8.t Array4.t, in_0:W32.t) : W8.t Array4.t = {
@@ -27,21 +27,6 @@ module M_Hop1(SC:Syscall_t) = {
     out <-
     Array4.init
     (WArray4.get8 (WArray4.set32_direct (WArray4.init8 (fun i => (out).[i])) 0 (in_0)));
-    return (out);
-  }
-
-  proc __ull_to_bytes_4 (out:W8.t Array4.t, in_0:W64.t) : W8.t Array4.t = {
-    var aux: int;
-
-    var i:int;
-
-    aux <- (- 1);
-    i <- (4 - 1);
-    while (aux < i) {
-      out.[i] <- (truncateu8 in_0);
-      in_0 <- (in_0 `>>` (W8.of_int 8));
-      i <- i - 1;
-    }
     return (out);
   }
 
@@ -67,6 +52,21 @@ module M_Hop1(SC:Syscall_t) = {
 
     aux <- (- 1);
     i <- (2 - 1);
+    while (aux < i) {
+      out.[i] <- (truncateu8 in_0);
+      in_0 <- (in_0 `>>` (W8.of_int 8));
+      i <- i - 1;
+    }
+    return (out);
+  }
+
+  proc __ull_to_bytes_4 (out:W8.t Array4.t, in_0:W64.t) : W8.t Array4.t = {
+    var aux: int;
+
+    var i:int;
+
+    aux <- (- 1);
+    i <- (4 - 1);
     while (aux < i) {
       out.[i] <- (truncateu8 in_0);
       in_0 <- (in_0 `>>` (W8.of_int 8));
@@ -171,19 +171,6 @@ module M_Hop1(SC:Syscall_t) = {
     return (a);
   }
 
-  proc __memset_u8_4 (a:W8.t Array4.t, value:W8.t) : W8.t Array4.t = {
-
-    var i:W64.t;
-
-    i <- (W64.of_int 0);
-
-    while ((i \ult (W64.of_int 4))) {
-      a.[(W64.to_uint i)] <- value;
-      i <- (i + (W64.of_int 1));
-    }
-    return (a);
-  }
-
   proc __memset_u8_128 (a:W8.t Array128.t, value:W8.t) : W8.t Array128.t = {
 
     var i:W64.t;
@@ -191,6 +178,19 @@ module M_Hop1(SC:Syscall_t) = {
     i <- (W64.of_int 0);
 
     while ((i \ult (W64.of_int 128))) {
+      a.[(W64.to_uint i)] <- value;
+      i <- (i + (W64.of_int 1));
+    }
+    return (a);
+  }
+
+  proc __memset_u8_4 (a:W8.t Array4.t, value:W8.t) : W8.t Array4.t = {
+
+    var i:W64.t;
+
+    i <- (W64.of_int 0);
+
+    while ((i \ult (W64.of_int 4))) {
       a.[(W64.to_uint i)] <- value;
       i <- (i + (W64.of_int 1));
     }
@@ -225,14 +225,14 @@ module M_Hop1(SC:Syscall_t) = {
     return (out);
   }
 
-  proc __memcpy_u8u8_32_32 (out:W8.t Array32.t, in_0:W8.t Array32.t) : 
-  W8.t Array32.t = {
+  proc __memcpy_u8u8_64_64 (out:W8.t Array64.t, in_0:W8.t Array64.t) : 
+  W8.t Array64.t = {
 
     var i:W64.t;
 
     i <- (W64.of_int 0);
 
-    while ((i \ult (W64.of_int 32))) {
+    while ((i \ult (W64.of_int 64))) {
       out.[(W64.to_uint i)] <- in_0.[(W64.to_uint i)];
       i <- (i + (W64.of_int 1));
     }
@@ -253,31 +253,17 @@ module M_Hop1(SC:Syscall_t) = {
     return (out);
   }
 
-  proc __memcpy_u8u8_64_64 (out:W8.t Array64.t, in_0:W8.t Array64.t) : 
-  W8.t Array64.t = {
+  proc __memcpy_u8u8_32_32 (out:W8.t Array32.t, in_0:W8.t Array32.t) : 
+  W8.t Array32.t = {
 
     var i:W64.t;
 
     i <- (W64.of_int 0);
 
-    while ((i \ult (W64.of_int 64))) {
+    while ((i \ult (W64.of_int 32))) {
       out.[(W64.to_uint i)] <- in_0.[(W64.to_uint i)];
       i <- (i + (W64.of_int 1));
     }
-    return (out);
-  }
-
-  proc _memcpy_u8u8_32_32 (out:W8.t Array32.t, in_0:W8.t Array32.t) : 
-  W8.t Array32.t = {
-
-    out <@ __memcpy_u8u8_32_32 (out, in_0);
-    return (out);
-  }
-
-  proc _memcpy_u8u8_64_32 (out:W8.t Array64.t, in_0:W8.t Array32.t) : 
-  W8.t Array64.t = {
-
-    out <@ __memcpy_u8u8_64_32 (out, in_0);
     return (out);
   }
 
@@ -288,12 +274,26 @@ module M_Hop1(SC:Syscall_t) = {
     return (out);
   }
 
-  proc _x_memcpy_u8u8_32_32 (out:W8.t Array32.t, in_0:W8.t Array32.t) : 
+  proc _memcpy_u8u8_64_32 (out:W8.t Array64.t, in_0:W8.t Array32.t) : 
+  W8.t Array64.t = {
+
+    out <@ __memcpy_u8u8_64_32 (out, in_0);
+    return (out);
+  }
+
+  proc _memcpy_u8u8_32_32 (out:W8.t Array32.t, in_0:W8.t Array32.t) : 
   W8.t Array32.t = {
+
+    out <@ __memcpy_u8u8_32_32 (out, in_0);
+    return (out);
+  }
+
+  proc _x_memcpy_u8u8_64_64 (out:W8.t Array64.t, in_0:W8.t Array64.t) : 
+  W8.t Array64.t = {
 
     out <- out;
     in_0 <- in_0;
-    out <@ _memcpy_u8u8_32_32 (out, in_0);
+    out <@ _memcpy_u8u8_64_64 (out, in_0);
     out <- out;
     return (out);
   }
@@ -308,12 +308,12 @@ module M_Hop1(SC:Syscall_t) = {
     return (out);
   }
 
-  proc _x_memcpy_u8u8_64_64 (out:W8.t Array64.t, in_0:W8.t Array64.t) : 
-  W8.t Array64.t = {
+  proc _x_memcpy_u8u8_32_32 (out:W8.t Array32.t, in_0:W8.t Array32.t) : 
+  W8.t Array32.t = {
 
     out <- out;
     in_0 <- in_0;
-    out <@ _memcpy_u8u8_64_64 (out, in_0);
+    out <@ _memcpy_u8u8_32_32 (out, in_0);
     out <- out;
     return (out);
   }
@@ -346,8 +346,8 @@ module M_Hop1(SC:Syscall_t) = {
     return (out);
   }
 
-  proc __memcpy_u8u8_2_32_2144 (out:W8.t Array32.t, in_0:W8.t Array2144.t,
-                                in_offset:W64.t, bytes:W64.t) : W8.t Array32.t *
+  proc __memcpy_u8u8_2_64_2144 (out:W8.t Array64.t, in_0:W8.t Array2144.t,
+                                in_offset:W64.t, bytes:W64.t) : W8.t Array64.t *
                                                                 W64.t = {
 
     var i:W64.t;
@@ -362,8 +362,8 @@ module M_Hop1(SC:Syscall_t) = {
     return (out, in_offset);
   }
 
-  proc __memcpy_u8u8_2_64_2144 (out:W8.t Array64.t, in_0:W8.t Array2144.t,
-                                in_offset:W64.t, bytes:W64.t) : W8.t Array64.t *
+  proc __memcpy_u8u8_2_32_2144 (out:W8.t Array32.t, in_0:W8.t Array2144.t,
+                                in_offset:W64.t, bytes:W64.t) : W8.t Array32.t *
                                                                 W64.t = {
 
     var i:W64.t;
@@ -832,8 +832,7 @@ module M_Hop1(SC:Syscall_t) = {
 
       ith_seed <- (Array32.init (fun i_0 => outseeds.[(i * 32) + i_0]));
 
-    aux_list <- _PRF_KEYGEN_ (to_list buf) (to_list inseed);
-    ith_seed <- Array32.of_list witness aux_list;
+    ith_seed <- _PRF_KEYGEN_ buf inseed;
 
       outseeds <- Array2144.init
                   (fun i_0 => if (i * 32) <= i_0 < (i * 32) + 32
@@ -1563,14 +1562,9 @@ module M_Hop1(SC:Syscall_t) = {
     var root:W8.t Array32.t;
     var i:W32.t;
     var idx_leaf:W32.t;
-    var _of_:bool;
-    var _cf_:bool;
-    var _sf_:bool;
-    var _zf_:bool;
     var wots_pk:W8.t Array2144.t;
     var leaf:W8.t Array32.t;
     var are_equal:W8.t;
-    var  _0:bool;
     buf <- witness;
     leaf <- witness;
     ltree_addr <- witness;
@@ -1618,7 +1612,7 @@ module M_Hop1(SC:Syscall_t) = {
 
       idx_leaf <- (W32.of_int ((1 `<<` 10) - 1));
       idx_leaf <- (idx_leaf `&` (truncateu32 idx));
-      (_of_, _cf_, _sf_,  _0, _zf_, idx) <- SHR_64 idx (W8.of_int 10);
+      idx <- (idx `>>` (truncateu8 ((W256.of_int 10) `&` (W256.of_int 63))));
 
       ots_addr <@ __set_layer_addr (ots_addr, i);
       ltree_addr <@ __set_layer_addr (ltree_addr, i);
@@ -1691,6 +1685,7 @@ module M_Hop1(SC:Syscall_t) = {
   W8.t Array32.t * W8.t Array320.t = {
     var aux: int;
 
+    var u:W32.t;
     var offset:W64.t;
     var ots_addr:W32.t Array8.t;
     var ltree_addr:W32.t Array8.t;
@@ -1702,7 +1697,6 @@ module M_Hop1(SC:Syscall_t) = {
     var buf:W8.t Array32.t;
     var heights:W32.t Array11.t;
     var t:W32.t;
-    var u:W32.t;
     var _of_:bool;
     var _cf_:bool;
     var _sf_:bool;
@@ -1722,6 +1716,7 @@ module M_Hop1(SC:Syscall_t) = {
     ltree_addr <- witness;
     node_addr <- witness;
     ots_addr <- witness;
+    u <- (W32.of_int 0);
     offset <- (W64.of_int 0);
 
     ots_addr <@ __zero_address_ (ots_addr);
@@ -1979,10 +1974,10 @@ module M_Hop1(SC:Syscall_t) = {
     var aux_0: W8.t Array128.t;
 
     var res_0:W64.t;
+    var exit_0:W8.t;
     var ots_addr:W32.t Array8.t;
     var t64:W64.t;
     var idx:W64.t;
-    var exit_0:W8.t;
     var idx_bytes:W8.t Array32.t;
     var sk_prf:W8.t Array32.t;
     var buf:W8.t Array32.t;
@@ -2014,6 +2009,7 @@ module M_Hop1(SC:Syscall_t) = {
     sk_prf <- witness;
     sk_seed <- witness;
 
+    exit_0 <- (W8.of_int 0);
     ots_addr <@ __zero_address_ (ots_addr);
     ots_addr <@ __set_type (ots_addr, (W32.of_int 0));
     _x__memcpy_u8pu8p (sm_ptr, (W64.of_int 2500), m_ptr, (W64.of_int 0),
